Busybeaver/Enumerate.lean
@@ -1,0 +1,213 @@
+/-
+How to enumerate turing machines.
+
+Note that we take heavy inspiration of busycoq here.
+-/
+
+import Mathlib.Tactic
+import Busybeaver.Basic
+import Busybeaver.Reachability
+
+namespace TM
+
+variable {M: Machine l s}
+
+namespace Machine
+
+inductive ZVisits (M: Machine l s): Label l → List (Label l) → Prop
+| halts : M q default = .halt → M.ZVisits q []
+| symNZ : ∀ q sym dir labh, M q default = .next sym dir labh → sym ≠ default → M.ZVisits q []
+| symZ : ∀ q dir nlab labt, M q default = .next default dir nlab → M.ZVisits nlab labt → M.ZVisits q (nlab :: labt)
+
+def equi_halts (M M': Machine l s) (c: Config l s): Prop := M.halts c ↔ M'.halts c
+
+namespace ZVisits
+
+lemma deterministic (h₁: M.ZVisits q L₁) (h₂: M.ZVisits q L₂): L₁ = L₂ :=
+  by induction h₁ generalizing L₂ with
+  | halts | symNZ => {
+    cases h₂ <;> simp_all
+  }
+  | symZ q dir nlab labt hqn _ IH₁ => {
+    induction h₂ with simp_all
+    | symZ q₂ dir₂ nlab₂ labt₂ _ v₂ => {
+      apply IH₁
+      exact v₂
+    }
+  }
+
+lemma in_split (h: M.ZVisits q L) (h': q' ∈ L): ∃n, M.ZVisits q' (L.drop (n + 1)) :=
+  by induction h with simp_all
+  | symZ q dir nlab labt qn v IH => {
+    rcases h' with h' | h'
+    swap
+    · obtain ⟨n, hn⟩ := IH h'
+      exists (n + 1)
+    by_contra hn
+    simp_all
+    specialize hn 0
+    simp_all
+  }
+
+lemma not_in (h: M.ZVisits q L): ¬(q ∈ L) :=
+  by {
+    intro hq
+    obtain ⟨n, hn⟩ := in_split h hq
+    have hLe := deterministic h hn
+    have hLl : L.length = (L.drop (n + 1)).length := by congr
+    rw [List.length_drop] at hLl
+    cases L with
+    | nil => contradiction
+    | cons he ta => {
+      suffices (he :: ta).length < (he :: ta).length by {
+        simp at this
+      }
+      calc (he :: ta).length
+      _ ≤ (he :: ta).length - (n + 1) := Nat.le_of_eq hLl
+      _ < (he :: ta).length := by {
+        apply Nat.sub_lt <;> simp
+      }
+    }
+  }
+
+lemma nodup (h: M.ZVisits q L): L.Nodup :=
+  by induction h with
+  | halts | symNZ => exact List.nodup_nil
+  | symZ _ _ nlab labt _ v IH => {
+    refine List.Nodup.cons ?symNZ.ha IH
+    exact not_in v
+  }
+
+lemma bound (h: M.ZVisits q L): L.length < Fintype.card (Label l) :=
+  by {
+    suffices L.toFinset.card < Fintype.card (Label l) by {
+      rw [Eq.symm (List.toFinset_card_of_nodup (nodup h))]
+      exact this
+    }
+    rw [← Finset.card_univ]
+    apply Finset.card_lt_card
+    constructor
+    · exact Finset.subset_univ L.toFinset
+    rw [Finset.not_subset]
+    exists q
+    constructor
+    · exact Finset.mem_univ q
+    · simp
+      exact not_in h
+  }
+
+lemma from_halts (hM: M.halts { state := q, tape := default }): ∃L, M.ZVisits q L :=
+  by {
+    let ⟨n, cfin, hcFin, hcR⟩ := hM
+    generalize h : Config.mk (s:=s) q default = C
+    simp_all
+    induction hcR generalizing q with
+    | refl => {
+      simp [Machine.LastState] at hcFin
+      apply Machine.step.none at hcFin
+      simp_all [default, ← h]
+      exists []
+      constructor
+      trivial
+    }
+    | @succ q' nxt C n step hn IH => {
+      simp_all [← h, -h]
+      simp [Machine.step] at step
+      split at step; simp at *
+      rename_i sym dir nlab hnlab
+
+      by_cases h_sym: sym = default
+      swap
+      · exists []
+        apply symNZ
+        · exact hnlab
+        · exact h_sym
+
+      suffices hL: ∃L, M.ZVisits nlab L by {
+        obtain ⟨L, hL⟩ := hL
+        exists nlab :: L
+        constructor
+        · simp_all
+          trivial
+        · exact hL
+      }
+
+      apply IH
+      · have hq : ⟨q, default⟩ -[M]-> nxt := by simp_all [Machine.step]
+        exact Machine.halts.tail (.single hq) hM
+
+      suffices hD: (Turing.Tape.write (Γ:=Symbol s) default default |>.move dir) = default by {
+        simp only [h_sym, hD] at step
+        cases step
+        rfl
+      }
+
+      suffices hCons: Turing.ListBlank.cons (Γ:=Symbol s) default default = default by {
+        cases dir <;> {
+          simp_all [Turing.Tape.move, Turing.Tape.write, hCons, default]
+          trivial
+        }
+      }
+
+      apply Turing.ListBlank.ext
+      intro i
+      induction i <;> {
+        simp
+        rfl
+      }
+    }
+    -- cases hcR with
+    -- | refl => {
+    -- }
+    -- | @succ _ nxt _ n stp hn => {
+    --   simp [Machine.step] at stp
+    --   simp [default] at hnlab
+    --   simp at *
+    --   by_cases h_sym: sym = default
+    --   swap
+    --   · exists []
+    --     apply Machine.ZVisits.symNZ
+    --     · exact hnlab
+    --     · exact h_sym
+
+    --   suffices hL: ∃ L, M.ZVisits nlab L by {
+    --     obtain ⟨L, hL⟩ := hL
+    --     exists nlab :: L
+    --     constructor
+    --     · simp_all
+    --       trivial
+    --     · exact hL
+    --   }
+
+    --   apply from_halts
+    --   apply halts.tail
+
+
+    --     -- apply from_halts
+    --     -- apply halts.tail
+    --     -- · apply Machine.Multistep.single (A:=?A) (by {
+    --     --     simp [Machine.step]
+    --     --   })
+    --     --   simp [Machine.step]
+    --     --   have hD:  := by {
+    --     --     unfold Turing.Tape.write
+    --     --     unfold Turing.Tape.move
+    --     --     intro L
+    --     --     sorry
+    --     --   }
+    --     -- · exact hM
+    --   }
+    -- }
+  }
+
+end ZVisits
+
+
+-- def ZVisits (M: Machine l s) (q: Label l): List (Label l) := match M q default with
+-- | .halt => []
+-- | .next sym dir q' => if sym = default then [] else q' :: (M.ZVisits q')
+-- termination_by M.ZVisitsP q
+-- decreasing_by {
+-- }
+
+end Machine
